ArkLib/OracleReduction/FiatShamir/DuplexSponge/Security/AbortAnalysis.lean
@@ -12,3 +12,11 @@ import ArkLib.OracleReduction.FiatShamir.DuplexSponge.Security.BadEvents
 This file contains the definition and analysis of aborts for the analysis of duplex sponge
 Fiat-Shamir, following Section 5.7 in the paper.
 -/
+
+/- Lemma 5.17: If `E(tr) = 0`, then `StdTrace(tr)` does not abort. -/
+
+/- Lemma 5.18: If `E(tr_𝒜) = 0`, then `𝒜 ^ D2SQuery` does not abort. -/
+
+/- Claim 5.19: If `E_inv(tr, s) = E_prp(tr) = E_fork(tr, s) = 0`, then `backTrack(tr, s) ≠ err`. -/
+
+/- Claim 5.20: If `E_prp(tr) = 0`, then `lookAhead(tr.p, s, i) ≠ err` for all `(s, i)`. -/
